core/modeling/ModelingSemantics.v
@@ -17,66 +17,47 @@ Section SemanticsModeling.
 
 Context {tc: TransformationConfiguration} {mtc: ModelingTransformationConfiguration tc}.  
 
-(* Fixpoint checkTypes (ses: list SourceElementType) (scs: list smmm.(EKind)) : bool :=
-  match ses, scs with
-  | se::ses', sc::scs' => 
-    match (toEData sc se) with
-    | Some c => checkTypes ses' scs'
-    | _ => false
-    end
-  | nil, nil => true
-  | _, _ => false
-  end. *) 
-
-(*
-Definition evalGuardExpr (r : ConcreteRule (smm:=smm)) (sm: SourceModel) (sp: list SourceElementType) : option bool :=
-  if (checkTypes sp (ConcreteRule_getInTypes (smm:=smm) r)) then
-    @evalGuardExpr' SourceElementType SourceModelLink TargetElementType TargetModelLink (parseRule r) sm sp
-  else Some false. *)
 
 (* ** Resolve *)
 
-(*Definition TraceLink' := @TraceLink SourceElementType TargetElementType.*)
 
 Local Notation TargetEKind := tmmm.(EKind).
 
-Definition denoteOutput (k: TargetEKind) (f: option TargetElementType): option (denoteEDatatype k) :=
-    match f with
-    | Some e => toEData k e
-    | _ => None
-    end.
+Definition denoteOutput (k: TargetEKind) (f: option TargetElementType) : option (denoteEDatatype k) := 
+  e <- f ; toEData k e.
 
 Definition denoteOutputList (k: TargetEKind) (f: option (list TargetElementType)): option (list (denoteEDatatype k)) :=
-    match f with
-    | Some l => Some (flat_map (fun e:TargetElementType => optionToList (toEData k e)) l)
-    | _ => None
-    end.
-
+  option_map 
+    (flat_map (fun e:TargetElementType => optionToList (toEData k e)))
+    f.
 
 Definition resolveIter (tls: list TraceLink) (sm: SourceModel) (name: string)
             (k: TargetEKind) (sp: list SourceElementType)
             (iter : nat) : option (denoteEDatatype k) :=
-  denoteOutput k (resolveIter tls sm name sp iter).
+  denoteOutput k (Semantics.resolveIter tls sm name sp iter).
 
 Definition resolve (tr: list TraceLink) (sm: SourceModel) (name: string)
   (k: TargetEKind) (sp: list SourceElementType) : option (denoteEDatatype k) :=
-  denoteOutput k (resolve tr sm name sp).
+  denoteOutput k (Semantics.resolve tr sm name sp).
 
 Definition resolveAllIter (tr: list TraceLink) (sm: SourceModel) (name: string)
   (k: TargetEKind) (sps: list(list SourceElementType)) (iter: nat)
   : option (list (denoteEDatatype k)) :=
-  denoteOutputList k (resolveAllIter tr sm name sps iter).
+  denoteOutputList k (Semantics.resolveAllIter tr sm name sps iter).
 
 Definition resolveAll (tr: list TraceLink) (sm: SourceModel) (name: string)
   (k: TargetEKind) (sps: list(list SourceElementType)) : option (list (denoteEDatatype k)) :=
-  denoteOutputList k (resolveAll tr sm name sps).
+  denoteOutputList k (Semantics.resolveAll tr sm name sps).
 
 Definition maybeResolve (tr: list TraceLink) (sm: SourceModel) (name: string)
   (k: TargetEKind) (sp: option (list SourceElementType)) : option (denoteEDatatype k) :=
-  denoteOutput k (maybeResolve tr sm name sp).
+  denoteOutput k (Semantics.maybeResolve tr sm name sp).
 
 Definition maybeResolveAll (tr: list TraceLink) (sm: SourceModel) (name: string)
   (k: TargetEKind) (sp: option (list (list SourceElementType))) : option (list (denoteEDatatype k)) :=
-  denoteOutputList k (maybeResolveAll tr sm name sp).
+  denoteOutputList k (Semantics.maybeResolveAll tr sm name sp).
 
 End SemanticsModeling.
+
+Ltac inv_denoteOutput H := monadInvN denoteOutput H.
+
