core/utils/OptionUtils.v
@@ -1,4 +1,5 @@
 Require Import String.
+Require Import NotationUtils.
 
 Definition is_option_eq 
   {A: Type} (oe : option A) 
@@ -21,3 +22,31 @@ Class ValueOption (A: Type) := {
 Instance ValueString : ValueOption string := {
    value (a: option string) := valueOption a ""%string
 }.
+
+
+Local Ltac inj H := injection H ; clear H ; intros ; subst.
+
+
+
+Ltac monadInv H :=
+  let N := fresh "E" in
+  
+  match type of H with 
+
+  |  _ <- ?E ; Some _ = Some _ => 
+      destruct E eqn:N ;
+      [ inj H | discriminate H ] ; 
+      let N2 := fresh H in
+      rename N into N2
+             
+  | _ <- ?E ; _ = Some _ => 
+      destruct E eqn:N ;
+      [  | discriminate H ]
+
+  | option_map _ _ = Some _ =>
+      unfold option_map in H ; monadInv H
+
+  end.
+
+Ltac monadInvN n H :=
+  unfold n in H ; monadInv H.
