transformations/Class2Relational/C2RTactics.v
@@ -67,7 +67,9 @@ Qed.
 
 Ltac unify_table_class_tac H :=
   match type of H with
-    In (TableElement ?ta) (instantiatePattern Class2Relational _ [ClassElement ?c]) => apply unify_table_class_lem in H ; subst ta
+    In (TableElement ?ta) (instantiatePattern Class2Relational _ [ClassElement ?c]) => 
+      apply unify_table_class_lem in H ;
+      subst ta
   end.
 
 Lemma unify_column_attribute_lem : 
@@ -83,21 +85,28 @@ Proof.
   auto.
 Qed.
 
+
 Ltac unify_column_attribute_tac H :=
-  let H2 := fresh in
   match type of H with 
     In (ColumnElement ?c)
       (instantiatePattern Class2Relational _
-         [AttributeElement ?a]) => apply unify_column_attribute_lem in H ; destruct H as [H2 H] ; subst c
+         [AttributeElement ?a]) => 
+      let H2 := fresh in
+      apply unify_column_attribute_lem in H ;
+      destruct H as [H2 H] ;
+      subst c
   end.
+
 
 Ltac unify_all :=
   match goal with
     [ H : In (ColumnElement _) (instantiatePattern Class2Relational _ [AttributeElement _]) |- _ ] =>
       unify_column_attribute_tac H
 
-   | [ H : In (TableElement _) (instantiatePattern Class2Relational _ [ClassElement _]) |- _ ] => unify_table_class_tac H
+   | [ H : In (TableElement _) (instantiatePattern Class2Relational _ [ClassElement _]) |- _ ] => 
+       unify_table_class_tac H
   end.
+
 
 Lemma make1 sm e :
   ConcreteExpressions.makeEmptyGuard [Class_K] sm [e] = true ->
@@ -105,6 +114,7 @@ Lemma make1 sm e :
 Proof.
   destruct e ; compute ; intro M ; [ eauto | discriminate].
 Qed.
+
 
 Lemma make1_alt sm e :
   ConcreteExpressions.makeEmptyGuard [Class_K] sm e = true ->
@@ -118,6 +128,7 @@ Proof.
       destruct s ; discriminate .
 Qed.
 
+
 Lemma make2 sm e:
   ConcreteExpressions.makeGuard [Attribute_K]
     (fun (_ : TransformationConfiguration.SourceModel)
@@ -129,6 +140,7 @@ Proof.
   destruct derived ; [ discriminate | ].
   eauto.
 Qed.
+
 
 Lemma make2_alt sm e:
   ConcreteExpressions.makeGuard [Attribute_K]
@@ -147,7 +159,6 @@ Proof.
 Qed.
 
 
-
 Ltac deduce_element_kind_from_guard :=
   let H2 := fresh "D" in
   let a := fresh "a" in
@@ -163,15 +174,16 @@ Ltac deduce_element_kind_from_guard :=
     (fun _ atr => negb (derived atr)) _ 
     [?e] = true |- _ ] =>
       apply make2 in H ; destruct H as (a & (H & H2)) ; 
-      first[ subst e (* if e was a variable *) 
-             | Tactics.inj H (* if e was not a variable *) ]
+      first[ 
+          subst e (* if e was a variable *) 
+        | Tactics.inj H (* if e was not a variable *) 
+        ]
 
-  | [ H :ConcreteExpressions.makeGuard [Attribute_K]
-    (fun _ atr => negb (derived atr)) _ 
-    ?e = true |- _ ] =>
-      apply make2_alt in H ; destruct H as (a & (H & H2)) ; 
-      (*first[*) subst e (* if e was a variable *) 
-             (*| Tactics.inj H (* if e was not a variable *) ]*)
+  | [ H :ConcreteExpressions.makeGuard [Attribute_K] (fun _ atr => negb (derived atr)) _  ?e = true |- _ ] =>
+      apply make2_alt in H ;
+      destruct H as (a & (H & H2)) ; 
+       subst e (* if e was a variable *) 
+             
 end.
 
 
@@ -189,13 +201,24 @@ Hint Resolve one_to_one : singleton_rules.
 
 (** ** Destructors *)
 
-Ltac destruct_In_two :=
+Lemma in_rules : forall r, 
+    In r (Syntax.rules Class2Relational) ->
+    r = core.modeling.Parser.parseRule Class2Relational.R1 \/ r = core.modeling.Parser.parseRule Class2Relational.R2.
+Proof.
+  unfold Class2Relational.
+  unfold Class2Relational'.
+  simpl.
+  intros ; auto.
+  repeat destruct_or H ; [ auto | auto | contradiction ].
+Qed.
+
+
+Ltac choose_rule :=
   match goal with 
     [ H : In ?X Class2Relational.(Syntax.rules) |- _ ] => 
-      simpl in H ; 
-      unfold In in H ; (* force it because simpl In can be disabled by Arguments In: simpl never. *)
-
-      repeat destruct_or H ; [ | | contradiction H] ; subst X
+      apply in_rules in H ;
+      destruct_or H ; 
+      subst X
   end.
 
 
@@ -207,7 +230,8 @@ Lemma allModelElements_allTuples e (cm:Model ClassMM):
   In [e] (allTuples Class2Relational cm).
 Proof. 
   intro.
-  apply (Tactics.allModelElements_allTuples (tc:=C2RConfiguration)); auto.
+  apply (Tactics.allModelElements_allTuples (tc:=C2RConfiguration));
+    auto.
 Qed.
 
 Lemma in_allTuples_singleton :
@@ -221,3 +245,64 @@ Proof.
   exact IN.
 Qed.
 
+(** *** January tactics *)
+
+
+Ltac progress_in_guard H :=
+  first [ progress unfold R1 in H | progress unfold R2 in H ] ;
+  Parser.unfold_parseRule H ; 
+  Tactics.simpl_accessors_any H ;
+  unfold Expressions.evalGuardExpr in H ;
+  Tactics.simpl_accessors_any H ;
+  deduce_element_kind_from_guard.
+
+
+Ltac progress_in_ope H ope :=
+  first [ progress unfold R1 in H | progress unfold R2 in H ] ;
+  Parser.unfold_parseRule H ; 
+  Tactics.simpl_accessors_any H ;
+  unfold map in H ; 
+  Tactics.simpl_accessors_any H ;
+  apply in_singleton in H ;
+  subst ope.
+
+
+Ltac progress_in_evalOutput H :=
+  unfold Expressions.evalOutputPatternElementExpr in H ;
+  Tactics.simpl_accessors_any H ;
+  unfold ConcreteExpressions.makeElement in H ;
+  unfold ConcreteExpressions.wrapElement in H ;
+  OptionUtils.monadInv H ;
+  simpl ConcreteExpressions.wrap in H ;
+  first [ discriminate | Tactics.inj H ].
+
+Ltac unfold_traceElementOnPattern H :=
+  match type of H with
+  | traceElementOnPattern _ _ _ _ = return _ => 
+      unfold traceElementOnPattern in H ; OptionUtils.monadInv H
+  end.
+
+Ltac progress_in_traceElementOnPattern H := 
+  unfold_traceElementOnPattern H ;
+  Tactics.unfold_instantiateElementOnPattern ; 
+  C2RTactics.progress_in_evalOutput H.
+
+
+Ltac unfold_toEData H :=
+  unfold toEData in H ;
+  simpl (unbox _) in H ;
+  unfold get_E_data in H.
+
+Ltac unfold_make_element H :=
+  unfold ConcreteExpressions.makeElement in H ;
+  unfold ConcreteExpressions.wrapElement in H ;
+  unfold ConcreteExpressions.wrap in H ;
+  unfold_toEData H ;
+  unfold ClassMetamodel.get_E_data in H.
+
+Ltac unfold_make_link H := 
+  unfold ConcreteExpressions.makeLink in H ;
+  unfold ConcreteExpressions.wrapLink in H ;
+  unfold ConcreteExpressions.wrap in H;
+  unfold_toEData H ;
+  unfold ClassMetamodel.get_E_data in H.
