transformations/Class2Relational/theorems/Column_name_uniqueness.v
@@ -22,7 +22,77 @@ Require Import transformations.Class2Relational.ClassMetamodel.
 Require Import transformations.Class2Relational.RelationalMetamodel.
 
 From transformations.Class2Relational 
-  Require C2RTactics.
+  Require C2RTactics Elements.
+
+
+Theorem Column_name_uniqueness_third_proof:
+forall (cm : ClassModel) (rm : RelationalModel), 
+    (* transformation *)
+    rm = execute Class2Relational cm ->
+    (* precondition *)
+    (forall (at1: Attribute_t) (at2: Attribute_t),
+        In (AttributeElement at1) cm.(modelElements) ->
+        In (AttributeElement at2) cm.(modelElements) ->
+
+        at1 <> at2 ->
+        attr_name at1 <> attr_name at2) ->
+    (* postcondition *)
+    (forall (co1: Column_t) (co2: Column_t),
+        In (ColumnElement co1) rm.(modelElements) ->
+        In (ColumnElement co2) rm.(modelElements) ->
+
+        co1 <> co2 ->
+        column_name co1 <> column_name co2).
+Proof.
+    intros cm rm E PRE co1 co2 IN1 IN2 D.
+    subst rm.
+
+    (* (0) *)
+    Tactics.chain_destruct_in_modelElements_execute.
+   
+    (* (1) *)
+    C2RTactics.choose_rule ; [ | ] ; 
+      
+      (* (2) *)
+      C2RTactics.progress_in_guard M;
+
+      (* (3) *)
+      C2RTactics.progress_in_ope IN_OP ope; 
+
+      (* (4) *)
+      C2RTactics.progress_in_evalOutput IN1 ; [ ]. 
+
+
+    (* (0) *)
+    Tactics.chain_destruct_in_modelElements_execute.
+    
+    (* (1) *)
+    C2RTactics.choose_rule ; [ | ]; 
+    
+    (* (2) *)
+      C2RTactics.progress_in_guard M;
+    
+
+      (* (3) *)
+      C2RTactics.progress_in_ope IN_OP ope; 
+
+      (* (4) *)
+      C2RTactics.progress_in_evalOutput IN2 ; []. 
+    
+    clear IN_I IN_I0.
+    
+    simpl.
+    destruct a ; destruct a0 ; simpl in * ; subst.
+    repeat Tactics.in_singleton_allTuples_auto.
+    
+    
+    specialize (PRE _ _ IN_E IN_E0). simpl in PRE. 
+    apply PRE.
+    
+    contradict D.
+    Tactics.inj D.
+    reflexivity.
+Qed.
 
 Theorem Column_name_uniqueness:
 forall (cm : ClassModel) (rm : RelationalModel), 
@@ -55,7 +125,7 @@ Proof.
     repeat C2RTactics.unify_all.
     simpl. 
     
-    repeat Tactics.in_singleton_allTuples.
+    repeat Tactics.in_singleton_allTuples_auto.
 
     specialize (PRE a a0 IN_E IN_E0). clear IN_E IN_E0.
 
@@ -66,6 +136,42 @@ Proof.
 Qed.
 
  
+(** An alternate proof based on simpler results. *)
+Theorem Column_name_uniqueness_alt_proof :
+forall (cm : ClassModel) (rm : RelationalModel), 
+    (* transformation *)
+    rm = execute Class2Relational cm ->
+    (* precondition *)
+    (forall (at1: Attribute_t) (at2: Attribute_t),
+        In (AttributeElement at1) cm.(modelElements) ->
+        In (AttributeElement at2) cm.(modelElements) ->
+
+        at1 <> at2 ->
+        attr_name at1 <> attr_name at2) ->
+    (* postcondition *)
+    (forall (co1: Column_t) (co2: Column_t),
+        In (ColumnElement co1) rm.(modelElements) ->
+        In (ColumnElement co2) rm.(modelElements) ->
+
+        co1 <> co2 ->
+        column_name co1 <> column_name co2).
+Proof.
+    intros cm rm E PRE co1 co2 IN1 IN2 D.
+    subst rm.
+    
+    destruct co1.
+    eapply Elements.transform_attribute_bw in IN1 ; [ | reflexivity ].
+
+    destruct co2.
+    eapply Elements.transform_attribute_bw in IN2 ; [ | reflexivity ].
+    
+    simpl.
+    
+    specialize (PRE _ _ IN1 IN2) ; clear IN1 IN2 ; simpl in PRE.
+
+    apply PRE ; clear PRE.
+    contradict D ; Tactics.inj D ; reflexivity.
+Qed.
 
 
   
