transformations/Class2Relational/theorems/Elements.v
@@ -1,0 +1,151 @@
+Require Import String.
+Require Import List.
+
+Require Import core.utils.Utils.
+Require Import core.Semantics.
+
+Require Import core.modeling.ModelingMetamodel.
+Require Import core.Model.
+
+Require Import transformations.Class2Relational.Class2Relational.
+Require Import transformations.Class2Relational.ClassMetamodel.
+Require Import transformations.Class2Relational.RelationalMetamodel.
+
+From transformations.Class2Relational 
+  Require ClassModelProperties RelationalModelProperties.
+
+From transformations.Class2Relational 
+  Require C2RTactics  TraceUtils.
+
+
+
+(** *** Utilities on transformation of elements *)
+
+
+Lemma transform_attribute_fw : 
+  forall (cm : ClassModel) (rm : RelationalModel), 
+  (* transformation *) rm = execute Class2Relational cm ->
+  (* precondition *)  forall id name,
+    In (AttributeElement {| attr_id:= id ; derived := false ; attr_name := name|}) cm.(modelElements) ->
+  (* postcondition *) 
+    In (ColumnElement {| column_id := id; column_name := name |}) (rm.(modelElements)). 
+Proof.
+  intros cm rm H ; subst.
+  intros i n H.
+  simpl.
+  apply C2RTactics.allModelElements_allTuples in H.
+  revert H ; generalize (allTuples Class2Relational cm).
+  induction l ; intro H ; [ solve [inversion H] | simpl ].
+  apply List.in_or_app.
+  simpl in H.
+  destruct_or H ; [ left | right ].
+  + subst.
+    clear IHl.
+    compute.
+    left.
+    reflexivity.
+  + auto. 
+Qed.
+
+
+Lemma transform_class_fw : 
+  forall (cm : ClassModel) (rm : RelationalModel), 
+  (* transformation *) rm = execute Class2Relational cm ->
+  (* precondition *)  forall id name,
+    In (ClassElement {| class_id:= id ; class_name := name|}) cm.(modelElements) ->
+  (* postcondition *) 
+    In (TableElement {| table_id := id; table_name := name |}) (rm.(modelElements)). 
+Proof.
+  intros cm rm H ; subst.
+  intros i n H.
+  simpl.
+  apply C2RTactics.allModelElements_allTuples in H.
+  revert H ; generalize (allTuples Class2Relational cm).
+  induction l ; intro H ; [ solve [inversion H] | simpl ].
+  apply List.in_or_app.
+  simpl in H.
+  destruct_or H ; [ left | right ].
+  + subst.
+    clear IHl.
+    compute.
+    left.
+    reflexivity.
+  + auto. 
+
+    (* Remark : exactly the same script as above. *)
+Qed.
+
+
+
+
+
+Lemma transform_attribute_bw : 
+  forall (cm : ClassModel) (rm : RelationalModel), 
+  (* transformation *) rm = execute Class2Relational cm ->
+  (* precondition *)  forall id name,
+      In (ColumnElement {| column_id := id; column_name := name |}) (rm.(modelElements)) ->
+  (* postcondition *) 
+    In (AttributeElement {| attr_id:= id ; derived := false ; attr_name := name|}) (cm.(modelElements))
+. 
+Proof.
+  intros cm rm H ; subst.
+  intros i n H.
+
+  (* (0) *)
+  Tactics.chain_destruct_in_modelElements_execute.
+  clear IN_I.
+
+  (* (1) To progress in M and H, we need to know ope, and so we need to know r. Exploit IN_R. *)
+
+  C2RTactics.choose_rule ; [ exfalso | ] ;
+
+  (* (2) Now to progress in M or H we need to know ope. Exploit M (guard). *) 
+
+  C2RTactics.progress_in_guard M ;
+
+
+  (* (3) make the ouput-pattern-element appear *)
+  C2RTactics.progress_in_ope IN_OP ope ;
+  
+  (* (4.E) make the matched element appear *)
+  C2RTactics.progress_in_evalOutput H.
+
+  apply Tactics.allModelElements_allTuples_back with (t:=Class2Relational).
+  destruct a. simpl in D. subst derived.  exact IN_E.
+  
+Qed.
+
+
+Lemma transform_class_bw : 
+  forall (cm : ClassModel) (rm : RelationalModel), 
+  (* transformation *) rm = execute Class2Relational cm ->
+  (* precondition *)  forall id name,
+      In (TableElement {| table_id := id; table_name := name |}) (rm.(modelElements)) ->
+  (* postcondition *) 
+    In (ClassElement {| class_id:= id ; class_name := name|}) (cm.(modelElements))
+. 
+Proof.
+  intros cm rm H ; subst.
+  intros i n H.
+
+  (* (0) *)
+  Tactics.chain_destruct_in_modelElements_execute.
+
+  clear IN_I.
+
+  (* (1) *)
+  C2RTactics.choose_rule ; [ | exfalso ];
+  
+  (* (2) *)
+  C2RTactics.progress_in_guard M ;
+
+  (* (3) *)
+  C2RTactics.progress_in_ope IN_OP ope ;
+  
+  (* (4.E) *)
+  C2RTactics.progress_in_evalOutput H.
+  
+  apply Tactics.allModelElements_allTuples_back with (t:=Class2Relational).
+  destruct x ; exact IN_E.
+
+Qed.
